use Kami word everywhere in end2end_lightbulb

end2end/src/End2EndLightbulb.v
@@ -3,18 +3,28 @@ Require Import Coq.Strings.String.
 Require Import Coq.Lists.List. Import ListNotations.
 Require Import coqutil.Word.Interface.
 Require Import coqutil.Map.Interface.
-Require Import end2end.End2EndPipeline.
 Require Import bedrock2.Syntax.
 Require Import bedrock2.Examples.lightbulb.
 Require Import bedrock2.TracePredicate. Import TracePredicateNotations.
-Require Import compiler.examples.integration.
 Require Import compiler.ProgramSpec.
 Require Import compiler.MemoryLayout.
+Require Import end2end.End2EndPipeline.
+Require Import end2end.Bedrock2SemanticsForKami.
 
 Open Scope Z_scope.
 Open Scope string_scope.
 
 Axiom TODO: False.
+
+Instance mapops: RegAlloc.map.ops (SortedListString.map Z). refine (
+  {| RegAlloc.map.intersect (s1 s2 : SortedListString.map Z) :=
+    {| SortedList.value := ListLib.list_intersect (fun '(k,v) '(k',v') => andb (_ k k') (_ v v')) (SortedList.value s1) (SortedList.value s2);
+       SortedList._value_ok := match TODO with end |};
+     RegAlloc.map.default_value := 666;
+  |}).
+- exact String.eqb.
+- exact Z.eqb.
+Defined.
 
 Definition instrMemSizeLg: Z := 10. (* TODO is this enough? *)
 Definition dataMemSize: Z := 4096.
@@ -58,10 +68,17 @@ Definition traceOfOneInteraction: list (lightbulb_spec.OP Semantics.word) -> Pro
 Definition goodHlTrace: list (lightbulb_spec.OP Semantics.word) -> Prop :=
   traceOfOneInteraction ^*.
 
+Definition relate_lightbulb_trace_to_bedrock(ioh: list (lightbulb_spec.OP Semantics.word))
+                                            (iol : Semantics.trace): Prop.
+  refine (SPI.mmio_trace_abstraction_relation (_ ioh) (_ iol)).
+  all: case TODO.
+  (* this should not be needed any more once lightbulb proofs are for generic word *)
+Defined.
+
 Definition spec: ProgramSpec := {|
   datamem_start := match TODO with end;
   datamem_pastend := match TODO with end;
-  goodTrace iol := exists ioh, SPI.mmio_trace_abstraction_relation ioh iol /\
+  goodTrace iol := exists ioh, relate_lightbulb_trace_to_bedrock ioh iol /\
                                goodHlTrace ioh;
   isReady t m l := exists buf R,
     (Separation.sep (Array.array Scalars.scalar8 (word.of_Z 1) (word.of_Z buffer_addr) buf) R) m /\
@@ -82,29 +99,17 @@ Lemma instrMemSizeLg_agrees_with_ml:
   word.sub (code_pastend ml) (code_start ml) = word.of_Z instrMemSizeLg.
 Admitted.
 
-Goal @Naive.rep 32 = Word.word 32.
-  (* TODO does not hold: bedrock2 separation logic word <> kami word !! *)
-Abort.
-
 Lemma end2end_lightbulb: False.
 Proof.
   pose proof link_lightbulb as P.
   unfold spec_of_iot in *.
 
   pose proof @end2end as Q.
-  specialize_first Q integration.mapops.
-
-  Fail specialize Q with (prog := prog).
-
-(*
- instrMemSizeLg
- dataMemSize
- prog
- spec
- ml
- mlOk
- memInit
- instrMemSizeLg_agrees_with_ml
-*)
+  specialize_first Q mapops.
+  specialize_first Q prog.
+  specialize_first Q instrMemSizeLg_agrees_with_ml.
+  specialize_first Q spec.
+  specialize_first Q mlOk.
+  specialize_first Q memInit.
 
 Abort.
