bedrock2/src/ChangeSemanticsParams.v
@@ -1,0 +1,68 @@
+Require Import Coq.ZArith.ZArith.
+Require Import bedrock2.Semantics.
+Require Import coqutil.Word.Interface.
+Require Import coqutil.Map.Interface.
+
+Open Scope Z_scope.
+
+Section Change.
+
+  Context {syntax : Syntax.parameters}
+          {varname_eqb : Syntax.varname -> Syntax.varname -> bool}
+          {funname_eqb : Syntax.funname -> Syntax.funname -> bool}
+          {actname_eqb : Syntax.actname -> Syntax.actname -> bool}
+          {width : BinNums.Z}
+          (wordA : word width)
+          (wordB : word width)
+          (byteA : word 8)
+          (byteB : word 8)
+          (memA : map.map wordA byteA)
+          (memB : map.map wordB byteB)
+          (localsA: map.map Syntax.varname wordA)
+          (localsB: map.map Syntax.varname wordB)
+          {funname_env : forall T : Type, map.map Syntax.funname T}.
+
+  Let traceA := list (memA * Syntax.actname * list wordA * (memA * list wordA)).
+  Let traceB := list (memB * Syntax.actname * list wordB * (memB * list wordB)).
+
+  Let ExtSpecA := traceA -> memA -> Syntax.actname -> list wordA ->
+                  (memA -> list wordA -> Prop) -> Prop.
+  Let ExtSpecB := traceB -> memB -> Syntax.actname -> list wordB ->
+                  (memB -> list wordB -> Prop) -> Prop.
+
+  Context {ext_specA : ExtSpecA}
+          {ext_specB : ExtSpecB}.
+
+  Instance p1: parameters := {
+    Semantics.syntax := syntax;
+    Semantics.varname_eqb := varname_eqb;
+    Semantics.funname_eqb := funname_eqb;
+    Semantics.actname_eqb := actname_eqb;
+    Semantics.width := width;
+    Semantics.word := wordA;
+    Semantics.byte := byteA;
+    Semantics.mem := memA;
+    Semantics.locals := localsA;
+    Semantics.funname_env := funname_env;
+    Semantics.ext_spec := ext_specA;
+  }.
+
+  Instance p2: parameters := {
+    Semantics.syntax := syntax;
+    Semantics.varname_eqb := varname_eqb;
+    Semantics.funname_eqb := funname_eqb;
+    Semantics.actname_eqb := actname_eqb;
+    Semantics.width := width;
+    Semantics.word := wordB;
+    Semantics.byte := byteB;
+    Semantics.mem := memB;
+    Semantics.locals := localsB;
+    Semantics.funname_env := funname_env;
+    Semantics.ext_spec := ext_specB;
+  }.
+
+  (* will need too many conversion functions/relations, don't do this, but generalize
+     program logic proofs to abstract word instance
+  Lemma change_params: exec
+  *)
+End Change.
