end2end/src/Bedrock2SemanticsForKami.v
@@ -1,0 +1,56 @@
+Require Import Coq.ZArith.ZArith.
+Require Import bedrock2.Syntax bedrock2.BasicCSyntax bedrock2.Semantics.
+Require coqutil.Datatypes.String coqutil.Map.SortedList coqutil.Map.SortedListString.
+Require Import coqutil.Word.Interface coqutil.Map.SortedListWord.
+Require Import coqutil.Z.HexNotation.
+Require Import processor.KamiWord.
+Require Import compiler.examples.MMIO.
+
+Import String List.ListNotations.
+Local Open Scope string_scope. Local Open Scope Z_scope. Local Open Scope list_scope.
+
+Definition MMIOREAD : string := "MMIOREAD".
+Definition MMIOWRITE : string := "MMIOWRITE".
+
+Instance word: word.word 32 := KamiWord.word 32.
+Instance byte: word.word 8 := KamiWord.word 8.
+
+Instance word_ok: word.ok word := KamiWord.ok 32 eq_refl.
+Instance byte_ok: word.ok byte := KamiWord.ok 8 eq_refl.
+
+
+Instance semantics: Semantics.parameters. refine ({|
+  width := 32;
+  syntax := StringNamesSyntax.make BasicCSyntax.StringNames_params;
+  varname_eqb := String.eqb;
+  funname_eqb := String.eqb;
+  actname_eqb := String.eqb;
+  mem := SortedListWord.map _ _;
+  locals := SortedListString.map _;
+  funname_env := SortedListString.map;
+  ext_spec := _;
+|}).
+unshelve refine (@MMIO.real_ext_spec {| MMIO.funname_env := SortedListString.map |}).
+eapply SortedListString.ok.
+Defined.
+
+Instance ok : Semantics.parameters_ok semantics.
+Proof.
+  split; cbv [funname_env locals mem semantics]; try exact _.
+  { cbv; auto. }
+  { eapply SortedListString.ok. }
+  { intros; eapply SortedListString.ok. }
+  (* case TODO. abstracting over TODO leads to untypable term! *)
+Admitted.
+
+(* TODO why does typeclass search fail here? *)
+Instance mapok: Interface.map.ok mem := SortedListWord.ok word _.
+
+Add Ring wring : (Properties.word.ring_theory (word := Semantics.word))
+      (preprocess [autorewrite with rew_word_morphism],
+       morphism (Properties.word.ring_morph (word := Semantics.word)),
+       constants [Properties.word_cst]).
+Add Ring bring : (Properties.word.ring_theory (word := Semantics.byte))
+      (preprocess [autorewrite with rew_word_morphism],
+       morphism (Properties.word.ring_morph (word := Semantics.byte)),
+       constants [Properties.word_cst]).
